src/TaggedNumbered.v
@@ -4,7 +4,7 @@ Require StepLib.
 Require Import Utopia.
 Require Import Monads.
 Require Import ListLemmas.
-Require HigherValue.
+Require Import HigherValue.
 
 
 Definition function_name := nat.
@@ -15,160 +15,101 @@ Definition function_name := nat.
 Definition rec_info := list bool.
 
 Inductive expr :=
+| Value (v : value)
 | Arg : expr
 | UpVar : nat -> expr
 | Call : expr -> expr -> expr
-| Constr (tag : nat) (args : list expr)
+| MkConstr (tag : nat) (args : list expr)
 | ElimN (n : nat) (cases : list (expr * rec_info)) (target : expr)
-| Close (f : function_name) (free : list expr)
+| MkClose (f : function_name) (free : list expr)
 .
 
 Definition env := list expr.
 
-Inductive value : expr -> Prop :=
-| VConstr : forall tag args, Forall value args -> value (Constr tag args)
-| VClose : forall f free, Forall value free -> value (Close f free).
-
-Section subst.
-Open Scope option_monad.
-
-Definition subst (arg : expr) (vals : list expr) (e : expr) : option expr :=
-    let fix go e :=
-        let fix go_list es : option (list expr) :=
-            match es with
-            | [] => Some []
-            | e :: es => cons <$> go e <*> go_list es
-            end in
-        (* NB: go_pair is non-recursive, but making it a fixpoint changes the
-         * behavior of `simpl` such that `refold` (below) works better. *)
-        let fix go_pair p : option (expr * rec_info) :=
-            let '(e, r) := p in
-            go e >>= fun e' => Some (e', r) in
-        let fix go_list_pair ps : option (list (expr * rec_info)) :=
-            match ps with
-            | [] => Some []
-            | p :: ps => cons <$> go_pair p <*> go_list_pair ps
-            end in
-        match e with
-        | Arg => Some arg
-        | UpVar n => nth_error vals n
-        | Call f a => Call <$> go f <*> go a
-        | Constr c es => Constr c <$> go_list es
-        | ElimN n cases target => ElimN n <$> go_list_pair cases <*> go target
-        | Close f free => Close f <$> go_list free
-        end in
-    go e.
-
-End subst.
+Inductive is_value : expr -> Prop :=
+| IsValue : forall v, is_value (Value v).
 
 
 Fixpoint unroll_elim (case : expr)
-                     (args : list expr)
+                     (args : list value)
                      (rec : rec_info)
                      (mk_rec : expr -> expr) : option expr :=
     match args, rec with
     | [], [] => Some case
     | arg :: args, r :: rec =>
-            let case := Call case arg in
-            let case := if r then Call case (mk_rec arg) else case in
+            let case := Call case (Value arg) in
+            let case := if r then Call case (mk_rec (Value arg)) else case in
             unroll_elim case args rec mk_rec
     | _, _ => None
     end.
 
-Inductive step (E : env) : expr -> expr -> Prop :=
-| MakeCall : forall f a free e e',
-    value a ->
-    Forall value free ->
-    nth_error E f = Some e ->
-    subst a free e = Some e' ->
-    step E (Call (Close f free) a) e'
-| CallL : forall e1 e1' e2,
-    step E e1 e1' ->
-    step E (Call e1 e2) (Call e1' e2)
-| CallR : forall v e2 e2',
-    value v ->
-    step E e2 e2' ->
-    step E (Call v e2) (Call v e2')
-| ConstrStep : forall tag vs e e' es,
-    step E e e' ->
-    Forall value vs ->
-    step E (Constr tag (vs ++ [e] ++ es)) (Constr tag (vs ++ [e'] ++ es))
-| ElimStep : forall n t t' cases,
-        step E t t' ->
-        step E (ElimN n cases t) (ElimN n cases t')
-| Eliminate : forall n tag args cases case rec e',
-    nth_error cases tag = Some (case, rec) ->
-    unroll_elim case args rec (fun x => ElimN n cases x) = Some e' ->
-    Forall value args ->
-    step E (ElimN n cases (Constr tag args)) e'
-| CloseStep : forall f vs e e' es,
-    step E e e' ->
-    Forall value vs ->
-    step E (Close f (vs ++ [e] ++ es)) (Close f (vs ++ [e'] ++ es))
+
+
+Inductive state :=
+| Run (e : expr) (l : list value) (k : value -> state)
+| Stop (v : value).
+
+Inductive sstep (E : env) : state -> state -> Prop :=
+| SArg : forall l k v,
+        nth_error l 0 = Some v ->
+        sstep E (Run Arg l k) (k v)
+| SUpVar : forall n l k v,
+        nth_error l (S n) = Some v ->
+        sstep E (Run (UpVar n) l k) (k v)
+
+| SCloseStep : forall tag vs e es l k,
+        Forall is_value vs ->
+        ~ is_value e ->
+        sstep E (Run (MkClose tag (vs ++ [e] ++ es)) l k)
+                (Run e l (fun v => Run (MkClose tag (vs ++ [Value v] ++ es)) l k))
+| SCloseDone : forall tag vs l k,
+        let es := map Value vs in
+        sstep E (Run (MkClose tag es) l k) (k (Close tag vs))
+
+| SConstrStep : forall fname vs e es l k,
+        Forall is_value vs ->
+        ~ is_value e ->
+        sstep E (Run (MkConstr fname (vs ++ [e] ++ es)) l k)
+                (Run e l (fun v => Run (MkConstr fname (vs ++ [Value v] ++ es)) l k))
+| SConstrDone : forall fname vs l k,
+        let es := map Value vs in
+        sstep E (Run (MkConstr fname es) l k) (k (Constr fname vs))
+
+| SCallL : forall e1 e2 l k,
+        ~ is_value e1 ->
+        sstep E (Run (Call e1 e2) l k)
+                (Run e1 l (fun v => Run (Call (Value v) e2) l k))
+| SCallR : forall e1 e2 l k,
+        is_value e1 ->
+        ~ is_value e2 ->
+        sstep E (Run (Call e1 e2) l k)
+                (Run e2 l (fun v => Run (Call e1 (Value v)) l k))
+| SMakeCall : forall fname free arg l k body,
+        nth_error E fname = Some body ->
+        sstep E (Run (Call (Value (Close fname free)) (Value arg)) l k)
+                (Run body (arg :: free) k)
+
+| SElimNStep : forall num cases target l k,
+        ~ is_value target ->
+        sstep E (Run (ElimN num cases target) l k)
+                (Run target l (fun v => Run (ElimN num cases (Value v)) l k))
+| SEliminate : forall num cases tag args l k case rec e',
+        nth_error cases tag = Some (case, rec) ->
+        unroll_elim case args rec (fun x => ElimN num cases x) = Some e' ->
+        sstep E (Run (ElimN num cases (Value (Constr tag args))) l k)
+                (Run e' l k)
 .
 
 
-(* Demo *)
 
-Definition add_lam_a :=             0.
-Definition add_lam_b :=             1.
-Definition elim_zero_lam_b :=       2.
-Definition elim_succ_lam_a :=       3.
-Definition elim_succ_lam_IHa :=     4.
-Definition elim_succ_lam_b :=       5.
+Definition sstar BE := StepLib.sstar (sstep BE).
+Definition SStarNil := @StepLib.SStarNil state.
+Definition SStarCons := @StepLib.SStarCons state.
 
-Definition add_reflect := Close add_lam_a [].
+Definition splus BE := StepLib.splus (sstep BE).
+Definition SPlusOne := @StepLib.SPlusOne state.
+Definition SPlusCons := @StepLib.SPlusCons state.
 
-Definition add_env : list expr :=
-    (* add_lam_a *)
-    [ Close add_lam_b [Arg]
-    (* add_lam_b *)
-    ; Call (ElimN 0
-        [(Close elim_zero_lam_b [Arg; UpVar 0], []);
-         (Close elim_succ_lam_a [Arg; UpVar 0], [true])] (UpVar 0)) Arg
-    (* elim_zero_lam_b *)
-    ; Arg
-    (* elim_succ_lam_a *)
-    ; Close elim_succ_lam_IHa [Arg; UpVar 0; UpVar 1]
-    (* elim_succ_lam_IHa *)
-    ; Close elim_succ_lam_b [Arg; UpVar 0; UpVar 1; UpVar 2]
-    (* elim_succ_lam_b *)
-    ; Call (UpVar 0) (Constr 1 [Arg])
-    ].
-
-Definition add_prog := (add_reflect, add_env).
-
-Inductive star (E : env) : expr -> expr -> Prop :=
-| StarNil : forall e, star E e e
-| StarCons : forall e e' e'',
-        step E e e' ->
-        star E e' e'' ->
-        star E e e''.
-
-Fixpoint nat_reflect n : expr :=
-    match n with
-    | 0 => Constr 0 []
-    | S n => Constr 1 [nat_reflect n]
-    end.
-
-Theorem add_1_2 : { x | star add_env
-        (Call (Call add_reflect (nat_reflect 1)) (nat_reflect 2)) x }.
-eexists.
-
-unfold add_reflect.
-eright. eapply CallL, MakeCall; try solve [repeat econstructor].
-eright. eapply MakeCall; try solve [repeat econstructor].
-eright. eapply CallL, Eliminate; try solve [repeat econstructor].
-  compute [unroll_elim ctor_arg_is_recursive].
-eright. eapply CallL, CallL, MakeCall; try solve [repeat econstructor].
-eright. eapply CallL, CallR, Eliminate; try solve [repeat econstructor].
-  compute [unroll_elim ctor_arg_is_recursive].
-eright. eapply CallL, MakeCall; try solve [repeat econstructor].
-eright. eapply MakeCall; try solve [repeat econstructor].
-eright. eapply MakeCall; try solve [repeat econstructor].
-eleft.
-Defined.
-(* Eval compute in proj1_sig add_1_2. *)
 
 
 (* Proofs *)
@@ -183,12 +124,13 @@ Definition expr_rect_mut
         (Pl : list expr -> Type)
         (Pp : expr * rec_info -> Type)
         (Plp : list (expr * rec_info) -> Type)
+    (HValue :   forall v, P (Value v))
     (HArg :     P Arg)
     (HUpVar :   forall n, P (UpVar n))
     (HCall :    forall f a, P f -> P a -> P (Call f a))
-    (HConstr :  forall tag args, Pl args -> P (Constr tag args))
+    (HConstr :  forall tag args, Pl args -> P (MkConstr tag args))
     (HElimN :   forall n cases target, Plp cases -> P target -> P (ElimN n cases target))
-    (HClose :   forall f free, Pl free -> P (Close f free))
+    (HClose :   forall f free, Pl free -> P (MkClose f free))
     (Hnil :     Pl [])
     (Hcons :    forall e es, P e -> Pl es -> Pl (e :: es))
     (Hpair :    forall e r, P e -> Pp (e, r))
@@ -210,108 +152,44 @@ Definition expr_rect_mut
             | p :: ps => Hcons_p p ps (go_pair p) (go_pair_list ps)
             end in
         match e as e_ return P e_ with
+        | Value v => HValue v
         | Arg => HArg
         | UpVar n => HUpVar n
         | Call f a => HCall f a (go f) (go a)
-        | Constr tag args => HConstr tag args (go_list args)
+        | MkConstr tag args => HConstr tag args (go_list args)
         | ElimN n cases target => HElimN n cases target (go_pair_list cases) (go target)
-        | Close f free => HClose f free (go_list free)
+        | MkClose f free => HClose f free (go_list free)
         end in go e.
 
 (* Useful wrapper for `expr_rect_mut with (Pl := Forall P)` *)
 Definition expr_ind' (P : expr -> Prop) (Pp : (expr * rec_info) -> Prop)
+    (HValue :   forall v, P (Value v))
     (HArg :     P Arg)
     (HUpVar :   forall n, P (UpVar n))
     (HCall :    forall f a, P f -> P a -> P (Call f a))
-    (HConstr :  forall c args, Forall P args -> P (Constr c args))
+    (HConstr :  forall c args, Forall P args -> P (MkConstr c args))
     (HElimN :   forall n cases target, Forall Pp cases -> P target -> P (ElimN n cases target))
-    (HClose :   forall f free, Forall P free -> P (Close f free))
+    (HClose :   forall f free, Forall P free -> P (MkClose f free))
     (Hpair :    forall e r, P e -> Pp (e, r))
     (e : expr) : P e :=
     ltac:(refine (@expr_rect_mut P (Forall P) Pp (Forall Pp)
-        HArg HUpVar HCall HConstr HElimN HClose _ _ Hpair _ _ e); eauto).
+        HValue HArg HUpVar HCall HConstr HElimN HClose _ _ Hpair _ _ e); eauto).
 
 (* Useful wrapper for `expr_rect_mut with (Pl := Forall P)` *)
 Definition expr_ind'' (P : expr -> Prop)
+    (HValue :   forall v, P (Value v))
     (HArg :     P Arg)
     (HUpVar :   forall n, P (UpVar n))
     (HCall :    forall f a, P f -> P a -> P (Call f a))
-    (HConstr :  forall c args, Forall P args -> P (Constr c args))
+    (HConstr :  forall c args, Forall P args -> P (MkConstr c args))
     (HElimN :   forall n cases target,
         Forall (fun c => P (fst c)) cases ->
         P target ->
         P (ElimN n cases target))
-    (HClose :   forall f free, Forall P free -> P (Close f free))
+    (HClose :   forall f free, Forall P free -> P (MkClose f free))
     (e : expr) : P e :=
     ltac:(refine (@expr_rect_mut P (Forall P) (fun c => P (fst c)) (Forall (fun c => P (fst c)))
-        HArg HUpVar HCall HConstr HElimN HClose _ _ _ _ _ e); eauto).
-
-
-(*
- * value_ok
- *)
-
-
-Inductive value_ok (E : env) : expr -> Prop :=
-| ConstrOk :
-        forall tag args,
-        Forall (value_ok E) args ->
-        value_ok E (Constr tag args)
-| CloseOk : forall f free body,
-        nth_error E f = Some body ->
-        Forall (value_ok E) free ->
-        value_ok E (Close f free).
-
-Theorem value_ok_value : forall E e, value_ok E e -> value e.
-induction e using expr_ind''; intro Hok; invc Hok.
-- constructor. list_magic_on (args, tt).
-- constructor. list_magic_on (free, tt).
-Qed.
-Hint Resolve value_ok_value.
-
-
-(*
- * Nested fixpoint aliases for subst
- *)
-
-Section subst_alias.
-Open Scope option_monad.
-
-Definition subst_list arg vals :=
-    let go := subst arg vals in
-    let fix go_list es : option (list expr) :=
-        match es with
-        | [] => Some []
-        | e :: es => cons <$> go e <*> go_list es
-        end in go_list.
-
-Definition subst_pair arg vals :=
-    let go := subst arg vals in
-    let fix go_pair p : option (expr * rec_info) :=
-        let '(e, r) := p in
-        go e >>= fun e' => Some (e', r) in go_pair.
-
-Definition subst_list_pair arg vals :=
-    let go_pair := subst_pair arg vals in
-    let fix go_list_pair ps : option (list (expr * rec_info)) :=
-        match ps with
-        | [] => Some []
-        | p :: ps => cons <$> go_pair p <*> go_list_pair ps
-        end in go_list_pair.
-
-End subst_alias.
-
-Ltac refold_subst arg vals :=
-    fold (subst_list arg vals) in *;
-    fold (subst_pair arg vals) in *;
-    fold (subst_list_pair arg vals) in *.
-
-Lemma subst_pair_fst : forall arg free p p',
-    subst_pair arg free p = Some p' ->
-    subst arg free (fst p) = Some (fst p').
-intros0 Hsub. destruct p. destruct p'. simpl in *.
-break_bind_option. inject_some. reflexivity.
-Qed.
+        HValue HArg HUpVar HCall HConstr HElimN HClose _ _ _ _ _ e); eauto).
 
 
 (*
@@ -325,96 +203,6 @@ first_induction args; destruct rec; intros; split; simpl;
 
 - intro Hlen. simpl. eapply IHargs. congruence.
 - intro Hcall. f_equal. apply <- IHargs. eauto.
-Qed.
-
-
-(*
- * Guaranteed success of subst
- *)
-
-Definition num_upvars :=
-    let fix go e :=
-        let fix go_list es :=
-            match es with
-            | [] => 0
-            | e :: es => max (go e) (go_list es)
-            end in
-        let fix go_pair p :=
-            match p with
-            | (e, _) => go e
-            end in
-        let fix go_list_pair ps :=
-            match ps with
-            | [] => 0
-            | p :: ps => max (go_pair p) (go_list_pair ps)
-            end in
-        match e with
-        | Arg => 0
-        | UpVar i => S i
-        | Call f a => max (go f) (go a)
-        | Constr _ args => go_list args
-        | ElimN _ cases target => max (go_list_pair cases) (go target)
-        | Close _ free => go_list free
-        end in go.
-
-(* Nested fixpoint aliases *)
-Definition num_upvars_list :=
-    let go := num_upvars in
-    let fix go_list es :=
-        match es with
-        | [] => 0
-        | e :: es => max (go e) (go_list es)
-        end in go_list.
-
-Definition num_upvars_pair :=
-    let go := num_upvars in
-    let fix go_pair (p : expr * rec_info) :=
-        match p with
-        | (e, _) => go e
-        end in go_pair.
-
-Definition num_upvars_list_pair :=
-    let go_pair := num_upvars_pair in
-    let fix go_list_pair ps :=
-        match ps with
-        | [] => 0
-        | p :: ps => max (go_pair p) (go_list_pair ps)
-        end in go_list_pair.
-
-Ltac refold_num_upvars :=
-    fold num_upvars_list in *;
-    fold num_upvars_pair in *;
-    fold num_upvars_list_pair in *.
-
-
-Lemma num_upvars_list_is_maximum : forall es,
-    num_upvars_list es = maximum (map num_upvars es).
-induction es; simpl in *; eauto.
-Qed.
-
-Lemma num_upvars_list_pair_is_maximum : forall ps,
-    num_upvars_list_pair ps = maximum (map num_upvars_pair ps).
-induction ps; simpl in *; eauto.
-Qed.
-
-Lemma num_upvars_list_le_Forall : forall es n,
-    num_upvars_list es <= n ->
-    Forall (fun e => num_upvars e <= n) es.
-intros.
-erewrite Forall_map with (P := fun x => x <= n).
-erewrite <- maximum_le_Forall.
-rewrite <- num_upvars_list_is_maximum.
-assumption.
-Qed.
-
-Lemma num_upvars_list_pair_le_Forall : forall es n,
-    num_upvars_list_pair es <= n ->
-    Forall (fun p => num_upvars_pair p <= n) es.
-intros.
-erewrite Forall_map with (P := fun x => x <= n).
-erewrite <- maximum_le_Forall.
-rewrite <- num_upvars_list_pair_is_maximum.
-assumption.
 Qed.
 
 
@@ -436,12 +224,13 @@ Definition num_locals :=
             | p :: ps => max (go_pair p) (go_list_pair ps)
             end in
         match e with
+        | Value _ => 0
         | Arg => 1
         | UpVar i => S (S i)
         | Call f a => max (go f) (go a)
-        | Constr _ args => go_list args
+        | MkConstr _ args => go_list args
         | ElimN _ cases target => max (go_list_pair cases) (go target)
-        | Close _ free => go_list free
+        | MkClose _ free => go_list free
         end in go.
 
 (* Nested fixpoint aliases *)
@@ -479,87 +268,6 @@ induction es; simpl in *; eauto.
 Qed.
 
 
-
-
-Lemma subst_list_is_map_partial : forall arg free es,
-    subst_list arg free es = map_partial (subst arg free) es.
-induction es.
-- reflexivity.
-- simpl. unfold seq, fmap, bind_option. simpl. repeat break_match; congruence.
-Qed.
-
-Lemma subst_list_pair_is_map_partial : forall arg free ps,
-    subst_list_pair arg free ps = map_partial (subst_pair arg free) ps.
-induction ps.
-- reflexivity.
-- simpl. unfold seq, fmap, bind_option. simpl. repeat break_match; congruence.
-Qed.
-
-Lemma Forall_subst_list_exists : forall arg free es,
-    Forall (fun e => exists e', subst arg free e = Some e') es ->
-    exists es', subst_list arg free es = Some es'.
-intros.
-rewrite subst_list_is_map_partial.
-eauto using map_partial_Forall_exists.
-Qed.
-
-Lemma Forall_subst_list_pair_exists : forall arg free es,
-    Forall (fun e => exists e', subst_pair arg free e = Some e') es ->
-    exists es', subst_list_pair arg free es = Some es'.
-intros.
-rewrite subst_list_pair_is_map_partial.
-eauto using map_partial_Forall_exists.
-Qed.
-
-
-
-Lemma num_upvars_subst : forall arg free body,
-    num_upvars body <= length free ->
-    exists body', subst arg free body = Some body'.
-induction body using expr_ind''; intros0 Hup;
-simpl in *; refold_num_upvars; refold_subst arg free.
-
-- eauto.
-
-- destruct (nth_error _ _) eqn:?; cycle 1.
-    { (* None *) rewrite nth_error_None in *. omega. }
-  eauto.
-
-- unfold seq, fmap.
-  destruct (nat_max_le ?? ?? ?? **).
-  specialize (IHbody1 **). destruct IHbody1 as [? HH1]. rewrite HH1.
-  specialize (IHbody2 **). destruct IHbody2 as [? HH2]. rewrite HH2.
-  simpl. eauto.
-
-- fwd eapply num_upvars_list_le_Forall; eauto.
-  fwd eapply Forall_subst_list_exists with (es := args).
-    { list_magic_on (args, tt). }
-  break_exists. find_rewrite. unfold seq, fmap. simpl. eauto.
-
-- destruct (nat_max_le _ _ _ **).
-
-  (* cases *)
-  fwd eapply num_upvars_list_pair_le_Forall; eauto.
-  fwd eapply Forall_subst_list_pair_exists with (es := cases).
-    { list_magic_on (cases, tt).
-      destruct cases_i. simpl in *.
-      fwd refine (_ _); try eassumption. break_exists. erewrite **.
-      simpl. eauto. }
-  break_exists. find_rewrite.
-
-  (* target *)
-  destruct (IHbody **). repeat find_rewrite.
-
-  unfold seq, fmap. simpl. eauto.
-
-- fwd eapply num_upvars_list_le_Forall; eauto.
-  fwd eapply Forall_subst_list_exists with (es := free0).
-    { list_magic_on (free0, tt). }
-  break_exists. find_rewrite. unfold seq, fmap. simpl. eauto.
-
-Qed.
-
-
 Lemma length_unroll_elim : forall case args rec mk_rec,
     length args = length rec ->
     exists e, unroll_elim case args rec mk_rec = Some e.
@@ -570,73 +278,6 @@ first_induction args; destruct rec; intros0 Hlen; simpl in Hlen; try discriminat
 Qed.
 
 
-(*
- * Validity of elim numbering
- *)
-
-Definition max_elim :=
-    let fix go e :=
-        let fix go_list es :=
-            match es with
-            | [] => 0
-            | e :: es => max (go e) (go_list es)
-            end in
-        let fix go_pair p :=
-            match p with
-            | (e, _) => go e
-            end in
-        let fix go_list_pair ps :=
-            match ps with
-            | [] => 0
-            | p :: ps => max (go_pair p) (go_list_pair ps)
-            end in
-        match e with
-        | Arg => 0
-        | UpVar _ => 0
-        | Call f a => max (go f) (go a)
-        | Constr _ args => go_list args
-        | ElimN n cases target => max n (max (go_list_pair cases) (go target))
-        | Close _ free => go_list free
-        end in go.
-
-(* Nested fixpoint aliases *)
-Definition max_elim_list :=
-    let go := max_elim in
-    let fix go_list es :=
-        match es with
-        | [] => 0
-        | e :: es => max (go e) (go_list es)
-        end in go_list.
-
-Definition max_elim_pair :=
-    let go := max_elim in
-    let fix go_pair (p : expr * rec_info) :=
-        match p with
-        | (e, _) => go e
-        end in go_pair.
-
-Definition max_elim_list_pair :=
-    let go_pair := max_elim_pair in
-    let fix go_list_pair ps :=
-        match ps with
-        | [] => 0
-        | p :: ps => max (go_pair p) (go_list_pair ps)
-        end in go_list_pair.
-
-Ltac refold_max_elim :=
-    fold max_elim_list in *;
-    fold max_elim_pair in *;
-    fold max_elim_list_pair in *.
-
-Lemma max_elim_list_is_maximum : forall es,
-    max_elim_list es = maximum (map max_elim es).
-induction es; simpl in *; eauto.
-Qed.
-
-Lemma max_elim_list_pair_is_maximum : forall ps,
-    max_elim_list_pair ps = maximum (map max_elim_pair ps).
-induction ps; simpl in *; eauto.
-Qed.
 
 
 (* Stricter validity of elim numbering *)
@@ -657,15 +298,16 @@ Definition elims_match elims : expr -> Prop :=
             | p :: ps => go_pair p /\ go_list_pair ps
             end in
         match e with
+        | Value _ => True
         | Arg => True
         | UpVar _ => True
         | Call f a => go f /\ go a
-        | Constr _ args => go_list args
+        | MkConstr _ args => go_list args
         | ElimN n cases target =>
                 nth_error elims n = Some cases /\
                 go_list_pair cases /\
                 go target
-        | Close _ free => go_list free
+        | MkClose _ free => go_list free
         end in go.
 
 Definition elims_match_list elims :=
@@ -722,6 +364,7 @@ induction e using expr_ind''; intros0 Helim;
 simpl in *; refold_elims_match elims; refold_elims_match (elims ++ elims').
 - constructor.
 - constructor.
+- constructor.
 - firstorder eauto.
 - rewrite elims_match_list_Forall in *. list_magic_on (args, tt).
 - destruct Helim as (? & ? & ?).  split; [|split].
@@ -755,404 +398,29 @@ list_magic_on (es, tt). eauto using elims_match_pair_extend.
 Qed.
 
 Lemma value_elims_match : forall elims v,
-    value v ->
+    is_value v ->
     elims_match elims v.
-induction v using expr_ind''; inversion 1; subst.
-- simpl. refold_elims_match elims. rewrite elims_match_list_Forall.
-  list_magic_on (args, tt).
-- simpl. refold_elims_match elims. rewrite elims_match_list_Forall.
-  list_magic_on (free, tt).
+intros0 Hval. invc Hval. constructor.
 Qed.
 
 Lemma unroll_elim_elims_match : forall elims case args rec mk_rec e',
     unroll_elim case args rec mk_rec = Some e' ->
     elims_match elims case ->
-    Forall (elims_match elims) args ->
     (forall e, elims_match elims e -> elims_match elims (mk_rec e)) ->
     elims_match elims e'.
-first_induction args; destruct rec; intros0 Hunroll Hcase Hargs Hmk_rec;
+first_induction args; destruct rec; intros0 Hunroll Hcase Hmk_rec;
 try discriminate; simpl in *.
 
 - inject_some. auto.
 
 - destruct b.
-  + on (Forall _ (_ :: _)), invc.
-    eapply IHargs; eauto.
+  + eapply IHargs; eauto.
     simpl. firstorder.
-  + on (Forall _ (_ :: _)), invc.
-    eapply IHargs; eauto.
+  + eapply IHargs; eauto.
     simpl. firstorder.
 Qed.
 
 
-
-(* Well-formedness *)
-
-Definition wf E : expr -> Prop :=
-    let fix go e :=
-        let fix go_list es :=
-            match es with
-            | [] => True
-            | e :: es => go e /\ go_list es
-            end in
-        let fix go_pair p :=
-            let '(e, _) := p in
-            go e in
-        let fix go_list_pair ps :=
-            match ps with
-            | [] => True
-            | p :: ps => go_pair p /\ go_list_pair ps
-            end in
-        match e with
-        | Arg => True
-        | UpVar _ => True
-        | Call f a => go f /\ go a
-        | Constr _ args => go_list args
-        | ElimN _ cases target => go_list_pair cases /\ go target
-        | Close fname free =>
-                (exists body,
-                    nth_error E fname = Some body /\
-                    num_upvars body <= length free) /\
-                go_list free
-        end in go.
-
-Definition wf_list E :=
-    let go := wf E in
-    let fix go_list es :=
-        match es with
-        | [] => True
-        | e :: es => go e /\ go_list es
-        end in go_list.
-
-Definition wf_pair E : (expr * rec_info) -> Prop :=
-    let go := wf E in
-    let fix go_pair p :=
-        let '(e, r) := p in
-        go e in go_pair.
-
-Definition wf_list_pair E :=
-    let go_pair := wf_pair E in
-    let fix go_list_pair ps :=
-        match ps with
-        | [] => True
-        | p :: ps => go_pair p /\ go_list_pair ps
-        end in go_list_pair.
-
-Ltac refold_wf E :=
-    fold (wf_list E) in *;
-    fold (wf_pair E) in *;
-    fold (wf_list_pair E) in *.
-
-
-
-
-(* closed terms *)
-
-Inductive closed : expr -> Prop :=
-| CCall : forall f a, closed f -> closed a -> closed (Call f a)
-| CConstr : forall tag args, Forall closed args -> closed (Constr tag args)
-| CElimN : forall num cases target,
-        Forall (fun p => closed (fst p)) cases ->
-        closed target ->
-        closed (ElimN num cases target)
-| CClose : forall fname free, Forall closed free -> closed (Close fname free)
-.
-
-Lemma subst_closed : forall arg upvars,
-    closed arg ->
-    Forall closed upvars ->
-    forall e e',
-    subst arg upvars e = Some e' ->
-    closed e'.
-intros0 Harg Hupvars.
-induction e using expr_rect_mut with
-    (Pl := fun es => forall es',
-        subst_list arg upvars es = Some es' ->
-        Forall closed es')
-    (Pp := fun p => forall p',
-        subst_pair arg upvars p = Some p' ->
-        closed (fst p'))
-    (Plp := fun ps => forall ps',
-        subst_list_pair arg upvars ps = Some ps' ->
-        Forall (fun p => closed (fst p)) ps');
-intros0 Hsubst; simpl in Hsubst; refold_subst arg upvars;
-break_bind_option; inject_some; inject_pair.
-
-- assumption.
-- eapply Forall_nth_error; eauto.
-- constructor; eauto.
-- constructor. eauto.
-- constructor; eauto.
-- constructor. eauto.
-
-- constructor.
-- constructor; eauto.
-
-- simpl. eauto.
-
-- constructor.
-- constructor; eauto.
-Qed.
-
-Lemma value_closed : forall e,
-    value e ->
-    closed e.
-induction e using expr_ind''; intros0 Hval; invc Hval.
-- constructor. list_magic_on (args, tt).
-- constructor. list_magic_on (free, tt).
-Qed.
-
-Lemma unroll_elim_closed : forall case args rec mk_rec e',
-    closed case ->
-    Forall closed args ->
-    (forall e, closed e -> closed (mk_rec e)) ->
-    unroll_elim case args rec mk_rec = Some e' ->
-    closed e'.
-first_induction args; destruct rec; simpl; intros0 Hcase Hargs Hmk_rec Helim; try discriminate.
-- inject_some. assumption.
-- invc Hargs.
-  eapply IHargs; [ .. | eassumption ]; try eassumption.
-  destruct b.
-  + constructor; [ constructor | ]; eauto.
-  + constructor; eauto.
-Qed.
-
-Lemma closed_step : forall E e e',
-    closed e ->
-    step E e e' ->
-    closed e'.
-induction e using expr_ind''; intros0 Hcl Hstep; invc Hcl; invc Hstep.
-
-- eapply subst_closed; [ .. | eassumption ].
-  + eauto using value_closed.
-  + list_magic_on (free, tt). eauto using value_closed.
-- constructor; eauto.
-- constructor; eauto.
-- on _, invc_using Forall_3part_inv.
-  on _, invc_using Forall_3part_inv.
-  constructor. eapply Forall_app; [ | constructor ]; eauto.
-- constructor; eauto.
-- eapply unroll_elim_closed; [ .. | eassumption ].
-  + fwd eapply Forall_nth_error; [ | eassumption | ]; eauto.
-  + list_magic_on (args, tt). eauto using value_closed.
-  + cbv beta. intros. constructor; eauto.
-- on _, invc_using Forall_3part_inv.
-  on _, invc_using Forall_3part_inv.
-  constructor. eapply Forall_app; [ | constructor ]; eauto.
-Qed.
-
-
-
-Inductive state :=
-| Run (e : expr) (l : list expr) (k : expr -> state)
-| Stop (e : expr).
-
-Inductive sstep (E : env) : state -> state -> Prop :=
-| SArg : forall l k v,
-        nth_error l 0 = Some v ->
-        sstep E (Run Arg l k) (k v)
-| SUpVar : forall n l k v,
-        nth_error l (S n) = Some v ->
-        sstep E (Run (UpVar n) l k) (k v)
-
-| SCloseStep : forall tag vs e es l k,
-        Forall value vs ->
-        ~ value e ->
-        sstep E (Run (Close tag (vs ++ [e] ++ es)) l k)
-                (Run e l (fun v => Run (Close tag (vs ++ [v] ++ es)) l k))
-| SCloseDone : forall tag vs l k,
-        Forall value vs ->
-        sstep E (Run (Close tag vs) l k) (k (Close tag vs))
-
-| SConstrStep : forall fname vs e es l k,
-        Forall value vs ->
-        ~ value e ->
-        sstep E (Run (Constr fname (vs ++ [e] ++ es)) l k)
-                (Run e l (fun v => Run (Constr fname (vs ++ [v] ++ es)) l k))
-| SConstrDone : forall fname vs l k,
-        Forall value vs ->
-        sstep E (Run (Constr fname vs) l k) (k (Constr fname vs))
-
-| SCallL : forall e1 e2 l k,
-        ~ value e1 ->
-        sstep E (Run (Call e1 e2) l k)
-                (Run e1 l (fun v => Run (Call v e2) l k))
-| SCallR : forall e1 e2 l k,
-        value e1 ->
-        ~ value e2 ->
-        sstep E (Run (Call e1 e2) l k)
-                (Run e2 l (fun v => Run (Call e1 v) l k))
-| SMakeCall : forall fname free arg l k body,
-        Forall value free ->
-        value arg ->
-        nth_error E fname = Some body ->
-        sstep E (Run (Call (Close fname free) arg) l k)
-                (Run body (arg :: free) k)
-
-| SElimNStep : forall num cases target l k,
-        ~ value target ->
-        sstep E (Run (ElimN num cases target) l k)
-                (Run target l (fun v => Run (ElimN num cases v) l k))
-| SEliminate : forall num cases tag args l k case rec e',
-        Forall value args ->
-        nth_error cases tag = Some (case, rec) ->
-        unroll_elim case args rec (fun x => ElimN num cases x) = Some e' ->
-        sstep E (Run (ElimN num cases (Constr tag args)) l k)
-                (Run e' l k)
-.
-
-
-
-Definition sstar BE := StepLib.sstar (sstep BE).
-Definition SStarNil := @StepLib.SStarNil state.
-Definition SStarCons := @StepLib.SStarCons state.
-
-Definition splus BE := StepLib.splus (sstep BE).
-Definition SPlusOne := @StepLib.SPlusOne state.
-Definition SPlusCons := @StepLib.SPlusCons state.
-
-
-
-Theorem add_1_2_s : { x | sstar add_env
-        (Run (Call (Call add_reflect (nat_reflect 1)) (nat_reflect 2)) [] Stop)
-        x }.
-eexists.
-
-unfold add_reflect.
-eright. eapply SCallL.
-  inversion 1.
-eright. eapply SMakeCall.
-  constructor.
-  repeat constructor.
-  reflexivity.
-eright. change [Arg] with ([] ++ [Arg] ++ []). eapply SCloseStep.
-  constructor.
-  inversion 1.
-eright. eapply SArg.
-  reflexivity.
-eright. eapply SCloseDone.
-  repeat constructor.
-eright. eapply SMakeCall.
-  repeat constructor.
-  repeat constructor.
-  reflexivity.
-eright. eapply SCallL.
-  inversion 1.
-eright. eapply SElimNStep.
-  inversion 1.
-eright. eapply SUpVar.
-  reflexivity.
-eright. eapply SEliminate.
-  repeat constructor.
-  reflexivity.
-  reflexivity.
-eright. eapply SCallL.
-  inversion 1.
-eright. eapply SCallL.
-  intros HH. invc HH. invc H0. invc H2.
-eright. change [Arg; UpVar 0] with ([] ++ [Arg] ++ [UpVar 0]). eapply SCloseStep.
-  constructor.
-  inversion 1.
-eright. eapply SArg.
-  reflexivity.
-eright. change ([] ++ [nat_reflect 2] ++ [UpVar 0]) with
-        ([nat_reflect 2] ++ [UpVar 0] ++ []). eapply SCloseStep.
-  repeat constructor.
-  inversion 1.
-eright. eapply SUpVar.
-  reflexivity.
-eright. eapply SCloseDone.
-  repeat constructor.
-eright. eapply SMakeCall.
-  repeat constructor.
-  repeat constructor.
-  reflexivity.
-Abort.
-
-Inductive flatten : state -> expr -> Prop :=
-| FRun : forall e a f k e' e'',
-        subst a f e = Some e' ->
-        flatten (k e') e''->
-        flatten (Run e (a :: f) k) e''
-| FStop : forall e,
-        flatten (Stop e) e.
-
-Inductive svalid : state -> Prop :=
-| VRun : forall e l k,
-        Forall value l ->
-        (forall v, value v -> svalid (k v)) ->
-        svalid (Run e l k)
-| VStop : forall v,
-        value v ->
-        svalid (Stop v).
-
-Lemma step_not_value : forall E e e',
-    step E e e' ->
-    ~ value e.
-induction e using expr_ind''; intros0 Hstep; invc Hstep;
-try solve [inversion 1].
-
-- inversion 1. subst.
-  invc_using Forall_3part_inv H.
-  invc_using Forall_3part_inv H3.
-  eapply H5; eauto.
-
-- inversion 1. subst.
-  invc_using Forall_3part_inv H.
-  invc_using Forall_3part_inv H3.
-  eapply H5; eauto.
-Qed.
-
-Inductive I : expr -> state -> Prop :=
-| IArg : forall l v k,
-        value v ->
-        nth_error l 0 = Some v ->
-        I v (Run Arg l k)
-| IUpVar : forall n l v k,
-        value v ->
-        nth_error l (S n) = Some v ->
-        I v (Run (UpVar n) l k)
-| ICall : forall f a f' a' l k,
-        I f (Run f' l k) ->
-        I a (Run a' l k) ->
-        I (Call f a) (Run (Call f' a') l k)
-| IConstr : forall tag args args' l k,
-        Forall2 (fun a a' => I a (Run a' l k)) args args' ->
-        I (Constr tag args) (Run (Constr tag args') l k)
-| IElimN : forall num cases target cases' target' l k,
-        Forall2 (fun c c' => I (fst c) (Run (fst c') l k)) cases cases' ->
-        I target (Run target' l k) ->
-        I (ElimN num cases target) (Run (ElimN num cases' target') l k)
-| IClose : forall fname free free' l k,
-        Forall2 (fun a a' => I a (Run a' l k)) free free' ->
-        I (Close fname free) (Run (Close fname free') l k)
-| IStop : forall v,
-        value v ->
-        I v (Stop v)
-.
-
-Lemma I_any_k : forall e e' l k k',
-    I e (Run e' l k) ->
-    I e (Run e' l k').
-induction e using expr_ind''; intros0 II.
-
-(* impossible - the first arg to `I` must always be a closed term *)
-- invc II; on (value _), invc.
-- invc II; on (value _), invc.
-
-- invc II; try on (value _), invc.
-  constructor; eauto.
-
-- invc II; constructor; eauto.
-  list_magic_on (args, (args', tt)).
-
-- invc II; try on (value _), invc.
-  constructor; eauto.
-  list_magic_on (cases, (cases', tt)).
-
-- invc II; constructor; eauto.
-  list_magic_on (free, (free', tt)).
-Qed.
 
 Require Import Metadata.
 Require Semantics.
@@ -1160,35 +428,21 @@ Require Semantics.
 Definition prog_type : Type := list expr * list metadata * list (list (expr * rec_info)) * list String.string.
 Definition valtype := HigherValue.value.
 
-Inductive expr_value : expr -> valtype -> Prop :=
-| EvConstr : forall tag args1 args2,
-        Forall2 expr_value args1 args2 ->
-        expr_value (Constr tag args1)
-                   (HigherValue.Constr tag args2)
-| EvClose : forall tag free1 free2,
-        Forall2 expr_value free1 free2 ->
-        expr_value (Close tag free1)
-                   (HigherValue.Close tag free2)
-.
-
 Definition initial_env (prog : prog_type) : env := fst (fst (fst prog)).
 
 Inductive is_callstate (prog : prog_type) : valtype -> valtype -> state -> Prop :=
-| IsCallstate : forall fname free free_e av ae body,
+| IsCallstate : forall fname free av body,
         nth_error (initial_env prog) fname = Some body ->
         let fv := HigherValue.Close fname free in
-        expr_value ae av ->
-        Forall2 expr_value free_e free ->
         HigherValue.public_value (snd (fst (fst prog))) fv ->
         HigherValue.public_value (snd (fst (fst prog))) av ->
         is_callstate prog fv av
-            (Run body (ae :: free_e) Stop).
+            (Run body (av :: free) Stop).
 
 Inductive final_state (prog : prog_type) : state -> valtype -> Prop :=
-| FinalState : forall e v,
-        expr_value e v ->
+| FinalState : forall v,
         HigherValue.public_value (snd (fst (fst prog))) v ->
-        final_state prog (Stop e) v.
+        final_state prog (Stop v) v.
 
 Definition semantics (prog : prog_type) : Semantics.semantics :=
   @Semantics.Semantics_gen state env valtype
@@ -1196,32 +450,3 @@ Definition semantics (prog : prog_type) : Semantics.semantics :=
                  (sstep)
                  (final_state prog)
                  (initial_env prog).
-
-
-
-Lemma expr_value_value : forall e v,
-    expr_value e v ->
-    value e.
-induction e using expr_rect_mut with
-    (Pl := fun es => forall vs,
-        Forall2 expr_value es vs ->
-        Forall value es)
-    (Pp := fun e => forall v,
-        expr_value (fst e) v ->
-        value (fst e))
-    (Plp := fun es => forall vs,
-        Forall2 (fun e v => expr_value (fst e) v) es vs ->
-        Forall (fun e => value (fst e)) es) ;
-intros0 Hev; try solve [invc Hev + simpl in *; eauto].
-
-- invc Hev. constructor. eauto.
-- invc Hev. constructor. eauto.
-Qed.
-Hint Resolve expr_value_value.
-
-Lemma expr_value_value_list : forall e v,
-    Forall2 expr_value e v ->
-    Forall value e.
-induction e; intros0 Hev; invc Hev; eauto using expr_value_value.
-Qed.
-Hint Resolve expr_value_value_list.
