src/UntypedComp8.v
@@ -11,10 +11,11 @@ Require Import CompilationUnit.
 Require Import Semantics.
 Require Import HighestValues.
 
-Require Untyped7.
+Require Untyped5.
 Require Untyped8.
 
-Module A := Untyped7.
+Module A := Untyped5.
+Module AS := Untyped4.
 Module B := Untyped8.
 
 
@@ -26,13 +27,14 @@ Definition compile_expr :=
             | e :: es => go e :: go_list es
             end in
         match e with
-        | A.Arg => B.Arg
-        | A.UpVar idx => B.UpVar idx
-        | A.App f a => B.App (go f) (go a)
-        | A.Constr ctor args => B.Constr ctor (go_list args)
-        | A.Close fname free => B.Close fname (go_list free)
-        | A.Elim ty cases target => B.Elim ty (go_list cases) (go target)
-        | A.OpaqueOp op args => B.Arg (* FIXME *)
+        | AS.Value v => B.Value v
+        | AS.Arg => B.Arg
+        | AS.UpVar idx => B.UpVar idx
+        | AS.App f a => B.App (go f) (go a)
+        | AS.MkConstr ctor args => B.MkConstr ctor (go_list args)
+        | AS.MkClose fname free => B.MkClose fname (go_list free)
+        | AS.Elim ty cases target => B.Elim ty (go_list cases) (go target)
+        | AS.OpaqueOp op args => B.Arg (* FIXME *)
         end in go.
 
 Definition compile_expr_list :=
@@ -45,74 +47,76 @@ Definition compile_expr_list :=
 
 Definition compile_genv := compile_expr_list.
 
-Definition compile_cu (cu : list A.expr * list metadata) :
+Definition compile_cu (cu : list AS.expr * list metadata) :
         list B.expr * list metadata :=
     let '(exprs, metas) := cu in
     (compile_genv exprs, metas).
 
 
-Inductive I_expr : A.expr -> B.expr -> Prop :=
-| IArg : I_expr (A.Arg) (B.Arg)
-| IUpVar : forall idx, I_expr (A.UpVar idx) (B.UpVar idx)
+Inductive I_expr : AS.expr -> B.expr -> Prop :=
+| IValue : forall v, I_expr (AS.Value v) (B.Value v)
+| IArg : I_expr (AS.Arg) (B.Arg)
+| IUpVar : forall idx, I_expr (AS.UpVar idx) (B.UpVar idx)
 | IApp : forall af aa bf ba,
         I_expr af bf ->
         I_expr aa ba ->
-        I_expr (A.App af aa) (B.App bf ba)
+        I_expr (AS.App af aa) (B.App bf ba)
 | IConstr : forall ctor aargs bargs,
         Forall2 I_expr aargs bargs ->
-        I_expr (A.Constr ctor aargs) (B.Constr ctor bargs)
+        I_expr (AS.MkConstr ctor aargs) (B.MkConstr ctor bargs)
 | IClose : forall fname afree bfree,
         Forall2 I_expr afree bfree ->
-        I_expr (A.Close fname afree) (B.Close fname bfree)
+        I_expr (AS.MkClose fname afree) (B.MkClose fname bfree)
 | IElim : forall ty acases atarget bcases btarget,
         Forall2 I_expr acases bcases ->
         I_expr atarget btarget ->
-        I_expr (A.Elim ty acases atarget) (B.Elim ty bcases btarget)
+        I_expr (AS.Elim ty acases atarget) (B.Elim ty bcases btarget)
 .
+Hint Resolve IValue.
 
-Inductive I_cont : A.cont -> (B.expr -> B.state) -> Prop :=
+Inductive I_cont : AS.cont -> (value -> B.state) -> Prop :=
 | IKAppL : forall ae2 al ak  be2 bl bk,
         I_expr ae2 be2 ->
-        Forall2 I_expr al bl ->
+        al = bl ->
         I_cont ak bk ->
-        I_cont (A.KAppL ae2 al ak) (fun v => B.Run (B.App v be2) bl bk)
+        I_cont (AS.KAppL ae2 al ak) (fun v => B.Run (B.App (B.Value v) be2) bl bk)
 | IKAppR : forall ae1 al ak  be1 bl bk,
         I_expr ae1 be1 ->
-        Forall2 I_expr al bl ->
+        al = bl ->
         I_cont ak bk ->
-        I_cont (A.KAppR ae1 al ak) (fun v => B.Run (B.App be1 v) bl bk)
+        I_cont (AS.KAppR ae1 al ak) (fun v => B.Run (B.App be1 (B.Value v)) bl bk)
 | IKConstr : forall ctor  avs aes al ak  bvs bes bl bk,
         Forall2 I_expr avs bvs ->
         Forall2 I_expr aes bes ->
-        Forall2 I_expr al bl ->
+        al = bl ->
         I_cont ak bk ->
-        I_cont (A.KConstr ctor avs aes al ak)
-               (fun v => B.Run (B.Constr ctor (bvs ++ v :: bes)) bl bk)
+        I_cont (AS.KConstr ctor avs aes al ak)
+               (fun v => B.Run (B.MkConstr ctor (bvs ++ B.Value v :: bes)) bl bk)
 | IKClose : forall fname  avs aes al ak  bvs bes bl bk,
         Forall2 I_expr avs bvs ->
         Forall2 I_expr aes bes ->
-        Forall2 I_expr al bl ->
+        al = bl ->
         I_cont ak bk ->
-        I_cont (A.KClose fname avs aes al ak)
-               (fun v => B.Run (B.Close fname (bvs ++ v :: bes)) bl bk)
+        I_cont (AS.KClose fname avs aes al ak)
+               (fun v => B.Run (B.MkClose fname (bvs ++ B.Value v :: bes)) bl bk)
 | IKElim : forall ty  acases al ak  bcases bl bk,
         Forall2 I_expr acases bcases ->
-        Forall2 I_expr al bl ->
+        al = bl ->
         I_cont ak bk ->
-        I_cont (A.KElim ty acases al ak)
-               (fun v => B.Run (B.Elim ty bcases v) bl bk)
-| IKStop : I_cont A.KStop B.Stop
+        I_cont (AS.KElim ty acases al ak)
+               (fun v => B.Run (B.Elim ty bcases (B.Value v)) bl bk)
+| IKStop : I_cont AS.KStop B.Stop
 .
 
-Inductive I : A.state -> B.state -> Prop :=
+Inductive I : AS.state -> B.state -> Prop :=
 | IRun : forall ae al ak  be bl bk,
         I_expr ae be ->
-        Forall2 I_expr al bl ->
+        al = bl ->
         I_cont ak bk ->
-        I (A.Run ae al ak) (B.Run be bl bk)
+        I (AS.Run ae al ak) (B.Run be bl bk)
 | IStop : forall av bv,
-        I_expr av bv ->
-        I (A.Stop av) (B.Stop bv)
+        av = bv ->
+        I (AS.Stop av) (B.Stop bv)
 .
 
 
@@ -121,9 +125,9 @@ Ltac i_ctor := intros; constructor; eauto.
 Ltac i_lem H := intros; eapply H; eauto.
 
 Lemma I_run_cont : forall av ak bv bk,
-    I_expr av bv ->
+    av = bv ->
     I_cont ak bk ->
-    I (A.run_cont ak av) (bk bv).
+    I (AS.run_cont ak av) (bk bv).
 intros0 IIval IIcont; invc IIcont; simpl; try solve [repeat i_ctor].
 - i_ctor. i_ctor. i_lem Forall2_app.
 - i_ctor. i_ctor. i_lem Forall2_app.
@@ -131,16 +135,15 @@ Qed.
 
 Lemma I_is_value : forall a b,
     I_expr a b ->
-    A.is_value a ->
+    AS.is_value a ->
     B.is_value b.
-mut_induction a using A.expr_rect_mut' with
+mut_induction a using AS.expr_rect_mut' with
     (Pl := fun as_ => forall bs,
         Forall2 I_expr as_ bs ->
-        Forall A.is_value as_ ->
+        Forall AS.is_value as_ ->
         Forall B.is_value bs);
 [ intros0 II Aval; invc II; invc Aval.. | ].
 
-- i_ctor.
 - i_ctor.
 
 - i_ctor.
@@ -154,15 +157,14 @@ Hint Resolve I_is_value_list.
 Lemma I_is_value' : forall b a,
     I_expr a b ->
     B.is_value b ->
-    A.is_value a.
+    AS.is_value a.
 mut_induction b using B.expr_rect_mut' with
     (Pl := fun bs => forall as_,
         Forall2 I_expr as_ bs ->
         Forall B.is_value bs ->
-        Forall A.is_value as_);
+        Forall AS.is_value as_);
 [ intros0 II Bval; invc II; invc Bval.. | ].
 
-- i_ctor.
 - i_ctor.
 
 - i_ctor.
@@ -173,7 +175,7 @@ Qed exporting.
 
 Lemma I_isnt_value : forall a b,
     I_expr a b ->
-    ~ A.is_value a ->
+    ~ AS.is_value a ->
     ~ B.is_value b.
 intros0 II Hnval. contradict Hnval. eauto using I_is_value'.
 Qed.
@@ -182,11 +184,11 @@ Hint Resolve I_isnt_value.
 
 Lemma I_unroll_elim' : forall acase bcase ctor aargs bargs amk_rec bmk_rec idx,
     I_expr acase bcase ->
-    Forall2 I_expr aargs bargs ->
+    aargs = bargs ->
     (forall a b, I_expr a b -> I_expr (amk_rec a) (bmk_rec b)) ->
-    I_expr (A.unroll_elim' acase ctor aargs amk_rec idx)
+    I_expr (AS.unroll_elim' acase ctor aargs amk_rec idx)
            (B.unroll_elim' bcase ctor bargs bmk_rec idx).
-first_induction aargs; intros0 IIcase IIargs IImk_rec; invc IIargs; simpl.
+first_induction aargs; intros0 IIcase IIargs IImk_rec; subst bargs; simpl.
 - assumption.
 - break_if.
   + eapply IHaargs; eauto. repeat i_ctor.
@@ -195,11 +197,22 @@ Qed.
 
 Lemma I_unroll_elim : forall acase bcase ctor aargs bargs amk_rec bmk_rec,
     I_expr acase bcase ->
-    Forall2 I_expr aargs bargs ->
+    aargs = bargs ->
     (forall a b, I_expr a b -> I_expr (amk_rec a) (bmk_rec b)) ->
-    I_expr (A.unroll_elim acase ctor aargs amk_rec)
+    I_expr (AS.unroll_elim acase ctor aargs amk_rec)
            (B.unroll_elim bcase ctor bargs bmk_rec).
 intros. eapply I_unroll_elim'; auto.
+Qed.
+
+
+Lemma I_expr_map_value : forall vs bes,
+    Forall2 I_expr (map AS.Value vs) bes ->
+    bes = map B.Value vs.
+induction vs; intros0 II; invc II.
+- reflexivity.
+- simpl. f_equal.
+  + on >I_expr, invc. reflexivity.
+  + apply IHvs. eauto.
 Qed.
 
 
@@ -215,12 +228,10 @@ intros0 Henv II Astep; inv Astep.
 all: invc II.
 all: try on (I_expr _ be), invc.
 
-- fwd eapply Forall2_nth_error_ex as HH; eauto.  destruct HH as (bv & ? & ?).
-  eexists. split. i_lem B.SArg.
+- eexists. split. i_lem B.SArg.
   i_lem I_run_cont.
 
-- fwd eapply Forall2_nth_error_ex as HH; eauto.  destruct HH as (bv & ? & ?).
-  eexists. split. i_lem B.SUpVar.
+- eexists. split. i_lem B.SUpVar.
   i_lem I_run_cont.
 
 
@@ -231,6 +242,7 @@ all: try on (I_expr _ be), invc.
   i_ctor. i_ctor.
 
 - on (I_expr _ bf), invc.
+  on (I_expr _ ba), invc.
   fwd eapply Forall2_nth_error_ex with (ys := BE) as HH; eauto.
     destruct HH as (bbody & ? & ?).
 
@@ -242,16 +254,18 @@ all: try on (I_expr _ be), invc.
   eexists. split. i_lem B.SConstrStep.
   i_ctor. i_ctor.
 
-- eexists. split. i_lem B.SConstrDone.
-  i_lem I_run_cont. i_ctor.
+- fwd eapply I_expr_map_value; eauto. subst.
+  eexists. split. i_lem B.SConstrDone.
+  i_lem I_run_cont.
 
 
 - on _, invc_using Forall2_3part_inv.
   eexists. split. i_lem B.SCloseStep.
   i_ctor. i_ctor.
 
-- eexists. split. i_lem B.SCloseDone.
-  i_lem I_run_cont. i_ctor.
+- fwd eapply I_expr_map_value; eauto. subst.
+  eexists. split. i_lem B.SCloseDone.
+  i_lem I_run_cont.
 
 
 - eexists. split. i_lem B.SElimTarget.
@@ -261,8 +275,6 @@ all: try on (I_expr _ be), invc.
   on (I_expr _ btarget), invc.
 
   eexists. split. i_lem B.SEliminate.
-  + on (constructor_arg_n _ = _), fun H => rewrite H.
-    i_lem Forall2_length.
   + i_ctor. i_lem I_unroll_elim. i_ctor.
 Qed.
 
@@ -273,7 +285,7 @@ Lemma admit_ A : A. Admitted.
 Lemma compile_I_expr : forall a b,
     compile_expr a = b ->
     I_expr a b.
-mut_induction a using A.expr_rect_mut' with
+mut_induction a using AS.expr_rect_mut' with
     (Pl := fun a => forall b,
         compile_expr_list a = b ->
         Forall2 I_expr a b);
@@ -302,42 +314,6 @@ Lemma compile_cu_metas : forall A Ameta B Bmeta,
 simpl. inversion 1. auto.
 Qed.
 
-Lemma I_expr_value : forall v a b,
-    I_expr a b ->
-    A.expr_value a v ->
-    B.expr_value b v.
-induction v using value_rect_mut with
-    (Pl := fun vs => forall as_ bs,
-        Forall2 I_expr as_ bs ->
-        Forall2 A.expr_value as_ vs ->
-        Forall2 B.expr_value bs vs);
-intros0 II Aev; invc Aev; invc II; i_ctor.
-Qed.
-
-Lemma A_expr_value_ex : forall v b,
-    B.expr_value b v ->
-    exists a, A.expr_value a v /\ I_expr a b.
-mut_induction v using value_rect_mut' with
-    (Pl := fun v => forall b,
-        Forall2 B.expr_value b v ->
-        exists a, Forall2 A.expr_value a v /\ Forall2 I_expr a b);
-[ intros0 Bev; invc Bev.. | ].
-
-- destruct (IHv ?? **) as (? & ? & ?).
-  eexists; split; i_ctor.
-
-- destruct (IHv ?? **) as (? & ? & ?).
-  eexists; split; i_ctor.
-
-- eexists; split; i_ctor.
-
-- destruct (IHv ?? **) as (? & ? & ?).
-  destruct (IHv0 ?? **) as (? & ? & ?).
-  eexists; split; i_ctor.
-
-- finish_mut_induction A_expr_value_ex using list.
-Qed exporting.
-
 Section Preservation.
 
     Variable aprog : A.prog_type.
@@ -357,13 +333,11 @@ Section Preservation.
     - simpl. intros0 Bcall Hf Ha. invc Bcall.
       fwd eapply Forall2_nth_error_ex' with (ys := B) as HH; eauto.
         destruct HH as (abody & ? & ?).
-      fwd eapply A_expr_value_ex as HH; eauto. destruct HH as (? & ? & ?).
-      fwd eapply A_expr_value_ex_list as HH; eauto. destruct HH as (? & ? & ?).
       eexists. split; repeat i_ctor.
 
     - simpl. intros0 II Afinal. invc Afinal. invc II.
 
-      eexists. split. i_ctor. i_lem I_expr_value. i_ctor.
+      eexists. split. i_ctor. reflexivity.
 
     - intros0 Astep. intros0 II.
       i_lem I_sim.
@@ -383,4 +357,3 @@ Section Preservation.
     Qed.
 
 End Preservation.
-
